heap_lang/heap.v
@@ -109,10 +109,10 @@ Section heap.
     heap_ctx ★ ▷ (∀ l, l ↦ v ={E}=★ Φ (LitV (LitLoc l))) ⊢ WP Alloc e @ E {{ Φ }}.
   Proof.
     iIntros (<-%of_to_val ?) "[#Hinv HΦ]". rewrite /heap_ctx.
-    iUpd (auth_empty heap_name) as "Ha".
-    iUpd (auth_open with "[$Hinv $Ha]") as (σ) "(%&Hσ&Hcl)"; first done.
-    iApply wp_alloc_pst. iFrame "Hσ". iNext. iIntros (l) "[% Hσ] !==>".
-    iUpd ("Hcl" with "* [Hσ]") as "Ha".
+    iMod (auth_empty heap_name) as "Ha".
+    iMod (auth_open with "[$Hinv $Ha]") as (σ) "(%&Hσ&Hcl)"; first done.
+    iApply wp_alloc_pst. iFrame "Hσ". iNext. iIntros (l) "[% Hσ] !>".
+    iMod ("Hcl" with "* [Hσ]") as "Ha".
     { iFrame. iPureIntro. rewrite to_heap_insert.
       eapply alloc_singleton_local_update; by auto using lookup_to_heap_None. }
     iApply "HΦ". by rewrite heap_mapsto_eq /heap_mapsto_def.
@@ -125,10 +125,10 @@ Section heap.
   Proof.
     iIntros (?) "[#Hinv [>Hl HΦ]]".
     rewrite /heap_ctx heap_mapsto_eq /heap_mapsto_def.
-    iUpd (auth_open with "[$Hinv $Hl]") as (σ) "(%&Hσ&Hcl)"; first done.
+    iMod (auth_open with "[$Hinv $Hl]") as (σ) "(%&Hσ&Hcl)"; first done.
     iApply (wp_load_pst _ σ); first eauto using heap_singleton_included.
-    iIntros "{$Hσ} !> Hσ !==>". iUpd ("Hcl" with "* [Hσ]") as "Ha"; first eauto.
-    by iApply "HΦ".
+    iIntros "{$Hσ}"; iNext; iIntros "Hσ !>".
+    iMod ("Hcl" with "* [Hσ]") as "Ha"; first eauto. by iApply "HΦ".
   Qed.
 
   Lemma wp_store E l v' e v Φ :
@@ -138,9 +138,9 @@ Section heap.
   Proof.
     iIntros (<-%of_to_val ?) "[#Hinv [>Hl HΦ]]".
     rewrite /heap_ctx heap_mapsto_eq /heap_mapsto_def.
-    iUpd (auth_open with "[$Hinv $Hl]") as (σ) "(%&Hσ&Hcl)"; first done.
+    iMod (auth_open with "[$Hinv $Hl]") as (σ) "(%&Hσ&Hcl)"; first done.
     iApply (wp_store_pst _ σ); first eauto using heap_singleton_included.
-    iIntros "{$Hσ} !> Hσ !==>". iUpd ("Hcl" with "* [Hσ]") as "Ha".
+    iIntros "{$Hσ}"; iNext; iIntros "Hσ !>". iMod ("Hcl" with "* [Hσ]") as "Ha".
     { iFrame. iPureIntro. rewrite to_heap_insert.
       eapply singleton_local_update, exclusive_local_update; last done.
       by eapply heap_singleton_included'. }
@@ -154,10 +154,10 @@ Section heap.
   Proof.
     iIntros (<-%of_to_val <-%of_to_val ??) "[#Hinv [>Hl HΦ]]".
     rewrite /heap_ctx heap_mapsto_eq /heap_mapsto_def.
-    iUpd (auth_open with "[$Hinv $Hl]") as (σ) "(%&Hσ&Hcl)"; first done.
+    iMod (auth_open with "[$Hinv $Hl]") as (σ) "(%&Hσ&Hcl)"; first done.
     iApply (wp_cas_fail_pst _ σ); [eauto using heap_singleton_included|done|].
-    iIntros "{$Hσ} !> Hσ !==>". iUpd ("Hcl" with "* [Hσ]") as "Ha"; first eauto.
-    by iApply "HΦ".
+    iIntros "{$Hσ}"; iNext; iIntros "Hσ !>".
+    iMod ("Hcl" with "* [Hσ]") as "Ha"; first eauto. by iApply "HΦ".
   Qed.
 
   Lemma wp_cas_suc E l e1 v1 e2 v2 Φ :
@@ -167,9 +167,9 @@ Section heap.
   Proof.
     iIntros (<-%of_to_val <-%of_to_val ?) "[#Hinv [>Hl HΦ]]".
     rewrite /heap_ctx heap_mapsto_eq /heap_mapsto_def.
-    iUpd (auth_open with "[$Hinv $Hl]") as (σ) "(%&Hσ&Hcl)"; first done.
+    iMod (auth_open with "[$Hinv $Hl]") as (σ) "(%&Hσ&Hcl)"; first done.
     iApply (wp_cas_suc_pst _ σ); first eauto using heap_singleton_included.
-    iIntros "{$Hσ} !> Hσ !==>". iUpd ("Hcl" with "* [Hσ]") as "Ha".
+    iIntros "{$Hσ}"; iNext; iIntros "Hσ !>". iMod ("Hcl" with "* [Hσ]") as "Ha".
     { iFrame. iPureIntro. rewrite to_heap_insert.
       eapply singleton_local_update, exclusive_local_update; last done.
       by eapply heap_singleton_included'. }
