program_logic/invariants.v
@@ -32,7 +32,7 @@ Proof. rewrite inv_eq /inv; apply _. Qed.
 Lemma inv_alloc N E P : ▷ P ={E}=★ inv N P.
 Proof.
   rewrite inv_eq /inv_def fupd_eq /fupd_def. iIntros "HP [Hw $]".
-  iUpd (ownI_alloc (∈ nclose N) P with "[HP Hw]") as (i) "(% & $ & ?)"; auto.
+  iMod (ownI_alloc (∈ nclose N) P with "[HP Hw]") as (i) "(% & $ & ?)"; auto.
   - intros Ef. exists (coPpick (nclose N ∖ coPset.of_gset Ef)).
     rewrite -coPset.elem_of_of_gset comm -elem_of_difference.
     apply coPpick_elem_of=> Hfin.
@@ -49,16 +49,16 @@ Proof.
   iDestruct "Hi" as % ?%elem_of_subseteq_singleton.
   rewrite {1 4}(union_difference_L (nclose N) E) // ownE_op; last set_solver.
   rewrite {1 5}(union_difference_L {[ i ]} (nclose N)) // ownE_op; last set_solver.
-  iIntros "(Hw & [HE $] & $)"; iUpdIntro; iApply except_0_intro.
+  iIntros "(Hw & [HE $] & $)"; iModIntro; iApply except_0_intro.
   iDestruct (ownI_open i P with "[Hw HE]") as "($ & $ & HD)"; first by iFrame.
-  iIntros "HP [Hw $] !==>"; iApply except_0_intro. iApply ownI_close; by iFrame.
+  iIntros "HP [Hw $] !> !>". iApply ownI_close; by iFrame.
 Qed.
 
 Lemma inv_open_timeless E N P `{!TimelessP P} :
   nclose N ⊆ E → inv N P ={E,E∖N}=★ P ★ (P ={E∖N,E}=★ True).
 Proof.
-  iIntros (?) "Hinv". iUpd (inv_open with "Hinv") as "[>HP Hclose]"; auto.
-  iIntros "!==> {$HP} HP". iApply "Hclose"; auto.
+  iIntros (?) "Hinv". iMod (inv_open with "Hinv") as "[>HP Hclose]"; auto.
+  iIntros "!> {$HP} HP". iApply "Hclose"; auto.
 Qed.
 End inv.
 
@@ -66,7 +66,7 @@ Tactic Notation "iInvCore" constr(N) "as" tactic(tac) constr(Hclose) :=
   let Htmp := iFresh in
   let patback := intro_pat.parse_one Hclose in
   let pat := constr:(IList [[IName Htmp; patback]]) in
-  iUpd (inv_open _ N with "[#]") as pat;
+  iMod (inv_open _ N with "[#]") as pat;
     [idtac|iAssumption || fail "iInv: invariant" N "not found"|idtac];
     [solve_ndisj || match goal with |- ?P => fail "iInv: cannot solve" P end
     |tac Htmp].
